## æ•™å¸ˆèŠ‚çš„è°¢ç¤¼ðŸ˜­

> ä¹ é¢˜äºŒ 1ï¼ˆ3ï¼‰ã€ï¼ˆ4ï¼‰ï¼›3ï¼›4ï¼ˆ3ï¼‰ã€ï¼ˆ4ï¼‰ï¼›6ï¼›7ï¼›8ï¼›9.

> [!exercise] 2.1 (3)

`BEGINPROOF`
$$\begin{align}
r(t)&=\left( a \frac{e^t+e^{-t}}{2},b \frac{e^t-e^{-t}}{2} \right) \\
\frac{\mathrm{d}r}{\mathrm{d}t}&=(a\sinh t,b\cosh t)\quad \frac{\mathrm{d}s}{\mathrm{d}t}= |r'(t)|=\sqrt{ \frac{a^2+b^2}{2}\cosh(2t)+\frac{a^2-b^2}{2} } \\
\mathrm{t}(s)&= \frac{\mathrm{d}r}{\mathrm{d}s}=\frac{\mathrm{d}r}{\mathrm{d}t} / \frac{\mathrm{d}s}{\mathrm{d}t}\quad n(s)=\begin{pmatrix}
0&-1 \\
1&0
\end{pmatrix}t(s) \\
\tiny \mathrm{t}'(s)& \tiny=\frac{\mathrm{d}\mathrm{ t}}{\mathrm{d}s}=\left( (a\cosh t,b\sinh t) \frac{\mathrm{d}t}{\mathrm{d}s}\times \frac{\mathrm{d}s}{\mathrm{d}t}+  (a\sinh t,b\cosh t) \frac{\mathrm{d}s}{\mathrm{d}t}\frac{1}{2\sqrt{ \frac{a^2+b^2}{2}\cosh(2t)+\frac{a^2-b^2}{2} }}\right) / \left( \frac{\mathrm{d}s}{\mathrm{d}t} \right)^2
\end{align}$$
ç”±äºŽ $\mathrm{t}'(s)\perp \mathrm{t}(s)$, ç”±å¾…å®šç³»æ•°æ³•


`ENDPROOF`